lean/kopis-spec.md
@@ -1,0 +1,274 @@
+# Kopis KEM Specification
+
+In this doc we define the Kopis key encapsulation mechanism (KEM). We do this in two parts, first defining an IND-CPA-secure public key encryption (PKE) scheme, then defining the IND-CCA-secure KEM via the Fujisaki-Okamoto transform.
+
+# Preliminaries
+
+We first specify all the algorithms, syntax, and mathematics we will need for the specification.
+
+## Dependencies
+
+We use the TurboSHAKE XOF family defined in [RFC 9861](https://www.rfc-editor.org/rfc/rfc9861.html). We invoke it as `TurboSHAKE128/TurboSHAKE256(M, L, D)`, where `M` is the message to be hashed, `L` is the desired output length, and `D` is the domain separator in the range `[0x01, 0x7f]`.
+
+The key words "MUST", "MUST NOT", "REQUIRED", "SHALL", "SHALL NOT", "SHOULD", "SHOULD NOT", "RECOMMENDED", "NOT RECOMMENDED", "MAY", and "OPTIONAL" in this document are to be interpreted as described in [BCP 14](https://www.rfc-editor.org/info/bcp14) [RFC 2119](https://www.rfc-editor.org/rfc/rfc2119.html) [RFC 8174](https://www.rfc-editor.org/rfc/rfc8174.html) when, and only when, they appear in all capitals, as shown here.
+
+## Syntax
+
+We use pseudocode resembling a mix of Rust and Python. Variables declared with `let mut` are mutable. Function definitions are preceded with `fn`, each function input name is followed by a colon, then the type signature, and each function  is followed by an arrow `->` then the return type. Ranges are denoted `a..b`, and indicate the range `[a, b)` (i.e., including `a`, excluding `b`). When `s` is a sequence type (e.g., a bitstring or bytestring), `s[a..b]` is used to denote the subsequence starting at index `a` (0-indexed), and ending at and excluding index `b`. We use underscores in the LHS of assignments to denote the elision of a value that is normally bound, e.g., `let (a, _) = f()` where `f()` returns two values. We use ellipses to denote the elision of multiple values, e.g., `let (a, ...) = f()`, where `f()` returns three values. We use infix `||` to denote concatenation of bytestrings. We use infix `^` to denote integer exponentiation when the inputs are expressions. We write `[uK; N]` to mean an array of `N` many `K`-bit integers. Subtraction over `uK` is always defined as wrapping subtraction, e.g., `0u8 - 1u8 = 255u8`.
+
+## Mathematical Definitions
+
+Let `R` be the negacyclic polynomial ring `ℤ[X]/(X²⁵⁶ + 1)`. We denote by `R13` the polynomial ring modulo `2^13`, i.e., `R/2¹³R` (this is isomorphic to `(ℤ/2¹³ℤ)[X]/(X²⁵⁶ + 1)`). Similarly, `R10` denotes `R/2¹⁰R` and `R1` denotes `R/2R`.
+
+The type `MatRn` refers to `Rn^(ℓ×ℓ)`, i.e., `ℓ×ℓ` matrices of elements of `Rn`, for any `n`. Similarly, the type `VecRn` refers to `Rn^ℓ`, i.e., vectors of `ℓ` elements of `Rn`. For any `n`, we write `make_rn` to refer to the natural morphism from the space of coefficients `[un; 256]` to `Rn` (input is interpreted lowest-degree-coefficient-first). `make_matn` takes a nested array `[[Rn; ℓ]; ℓ]` and interprets it as a list of rows in a matrix in `MatRn`. `make_vecn` takes an array `[Rn; ℓ]` and interprets it as a column vector in `VecRn`, in the same order as `make_matn`, i.e., such that `make_matn([eye, zeros, ... zeros]) * make_vecn(eye) = make_vecn(eye)`, where `eye = [1, 0, ..., 0]` , and `zeros = [0, 0, ..., 0]` (interpreting the numbers as ring elements). When indexing into a vector `v: VecRn` for some `n`, we do so in the same order that was used in its constructor, i.e., `v[i]` equals `a[i]` where `a` is the input to the `make_vecn` that constructed `v`. `transpose` transposes the given matrix or vector. 
+
+When we write `r as U` for some type `U`, we mean to invoke either the natural injection or projection of `r` into/onto `U`. For example, if `r` is in `VecR10` and `U` is `VecR13`, then it is the natural injection, and if vice-versa, then it is the natural projection by quotienting by `2¹⁰R13`.
+
+For any modulus `N`, we say the canonical form of an element of `ℤ/Nℤ` is its representative integer in `[0, N)`. For any `n` and a ring element `r` we say its _canonical coefficients_ `canonical_coeffs(r: Rn) -> [un; 256]` are the unique sequence of 256 `un` values `a_0, ..., a_255` such that `r = a_255 X^255 + ... + a_1 X + a_0`.
+
+For an element `r` in `Rn` and integer `N`, we define the right-shift `r >> N` as `make_rn([a_0 >> N, a_1 >> N, ..., a_255 >> N])` where `a_i` are the canonical coefficients of `r`. We define left-shift `r << N` similarly, with coefficients reduced mod `2^n`. We define right and left shift for elements of `VecRn` as operating element-wise.
+
+We define `to_bits_le(n: ℤ, k: un) -> [bool; n]` to be the function that converts an `n`-bit integer to its bit representation, starting with the least significant bit. Similarly, we define 
+`from_bits_le(n: ℤ, bits: [bool; n]) -> un` to interpret `n` bits as a `un` value, using `bits[0]` as the least significant bit of the output, and so on.
+
+# Main Algorithms
+
+We now define a **public key encryption (PKE) scheme**. For the purposes of this specification, the secret key space is simply `[u8; 32]`, and generating a fresh secret key amounts to generating a fresh uniform bytestring. We define a public key encryption scheme as the set of the following algorithms:
+
+* `SkToPk(sk) -> pk` — Computes the public key corresponding to the given secret key
+* `PkeEncrypt(randomness, pk, msg) -> ct` — Encrypts the given message `msg` to public key `pk`, using encryption randomness `randomness`
+* `PkeDecrypt(sk, ct) -> msg` — Decrypts the given ciphertext `ct` using the secret key `sk`, and unconditionally returns a message `msg`
+
+We now define a **key encapsulation mechanism (KEM)**. Similar to the PKE above, secret keys are uniform elements of `[u8; 32]`. A KEM is defined as the set of the following algorithms:
+
+* `SkToPk(sk) -> pk` — Computes the public key corresponding to the given secret key
+* `KemEncap(randomness, pk) -> (k, ct)` — Encapsulates a shared secret `k` to public key `pk`, using randomness `randomness`. Outputs a `k` and a ciphertext `ct`.
+* `KemDecap(sk, ct) -> k` — Decrypts the ciphertext `ct` using the secret key `sk`, and unconditionally returns a shared secret `k`
+
+For real-world usage of these algorithms, the `randomness` parameters above MUST be sampled uniformly.
+
+An implementation note: the purpose of Kopis is to be used in settings that require constant-time operations. Thus, any implementation of the above functions MUST be constant-time with respect to all inputs.
+
+## Parameters
+
+The following variables represent security parameters, and depend on the security level being instantiated:
+
+* `ℓ` — The public matrix dimension. This impacts the size of public keys and ciphertexts
+* `μ` — The binomial parameter used for secret generation. This is always even.
+* `t` — The base-2 logarithm of the modulus of the space of compressed ring elements
+
+## Constants
+
+We define the constants used in our implementation. The size in bytes of our secret keys, public keys, and ciphertexts are functions of the parameters above:
+
+* `SK_SIZE = 32`
+* `PK_SIZE = 256*ℓ*10/8 + 32`
+* `CT_SIZE = 256*t/8 + 256*ℓ*10/8`
+
+We also require domain separators for all our TurboSHAKE invocations:
+
+* `DOMSEP_KGEXPAND = 0x01`
+* `DOMSEP_GENMAT = 0x02`
+* `DOMSEP_GENSEC = 0x03`
+* `DOMSEP_PKHASH = 0x04`
+* `DOMSEP_FO = 0x05`
+* `DOMSEP_NOREJECT = 0x06`
+
+## PKE
+
+We define key generation, encryption, and decryption for the Kopis IND-CPA-secure PKE scheme. We will define the helper functions later.
+
+```
+fn SkToPk(sk: [u8; 32]) -> [u8; PK_SIZE]:
+  let (_, _, pk, _) = ExpandSecretKey(sk)
+  return pk
+
+fn PkeEncrypt(
+  randomness: [u8; 32],
+  pk: [u8; PK_SIZE],
+  msg: [u8; 32]
+) -> [u8; CT_SIZE]:
+  let vec_b = deserialize_vec(10, pk[..256*ℓ*10/8])
+  let mat_seed = pk[256*ℓ*10/8..]
+  let m = deserialize_elem(1, msg)
+
+  let mat_A = GenMat(mat_seed)
+  let vec_sprime = GenSecret(randomness)
+  let vec_bprime = CompressToR10(mat_A * vec_sprime)
+  let vprime = transpose(vec_b) * (vec_sprime as VecR10)
+  let cm = CompressToRt(vprime - ((m as R10) << 9))
+
+  let ct = serialize_vec(10, vec_bprime) || serialize_elem(t, cm)
+  return ct
+
+fn PkeDecrypt(sk: [u8; 32], ct: [u8; CT_SIZE]) -> [u8; 32]:
+  let (vec_s, ...) = ExpandSecretKey(sk)
+  let vec_bprime = deserialize_vec(10, ct[..256*ℓ*10/8])
+  let cm = deserialize_elem(t, ct[256*ℓ*10/8..])
+  let v = transpose(vec_bprime) * (vec_s as VecR10)
+  let cm10 = (cm as R10) << (10 - t)
+  let mprime = DecodeMsg(v - cm10)
+  return serialize_elem(1, mprime)
+```
+
+## KEM
+
+We define the IND-CCA-secure Kopis KEM below. The `SkToPk` function is identical to the one given in the PKE above.
+
+```
+fn KemEncap(
+  randomness: [u8; 32],
+  pk: [u8; PK_SIZE]
+) -> ([u8; 32], [u8; CT_SIZE]):
+  # Derive the output key and encryption randomness
+  let pkh = TurboSHAKE256(pk, 32, DOMSEP_PKHASH)
+  let b = TurboSHAKE256(randomness || pkh, 64, DOMSEP_FO)
+  let (k, r) = (b[..32], b[32..])
+
+  # Encrypt to pk. `randomness` is itself the message
+  let ct = PkeEncrypt(r, pk, randomness)
+
+  return (k, ct)
+
+fn KemDecap(sk: [u8; 32], ct: [u8; CT_SIZE]) -> [u8; 32]:
+  let (_, z, pk, pkh) = ExpandSecretKey(sk)
+
+  let randomness = PkeDecrypt(sk, ct)
+  let b = TurboSHAKE256(randomness || pkh, 64, DOMSEP_FO)
+  let (k, rprime) = (b[..32], b[32..])
+  let cprime = PkeEncrypt(rprime, pk, randomness)
+
+  if ct == cprime:
+    return k
+  else:
+    return TurboSHAKE256(z || ct, 32, DOMSEP_NOREJECT)
+```
+
+We note again that, along with all other top-level functions, `KemDecap` MUST be constant time with respect to its inputs. In particular, an implementer MUST perform the ciphertext equality check in constant time.
+
+For efficiency, implementers MAY internally cache the expanded decapsulation key. But this expanded key SHOULD NOT be persisted anywhere.
+
+## Auxiliary Functions
+
+We now define the auxiliary functions used in the schemes above:
+
+```
+fn ExpandSecretKey(
+  sk: [u8; 32]
+) -> (VecR13, [u8; 32], [u8; PK_SIZE], [u8; 32]):
+  let randomness = TurboSHAKE256(sk || (ℓ as u8), 96, DOMSEP_KGEXPAND)
+  let mat_seed = randomness[..32]
+  let secret_seed = randomness[32..64]
+  let z = randomness[64..]
+
+  let mat_A = GenMat(mat_seed)
+  let vec_s = GenSecret(secret_seed)
+  let vec_b = CompressToR10(transpose(mat_A) * vec_s)
+  let pk = serialize_vec(10, vec_b) || mat_seed
+  let pkh = TurboSHAKE256(pk, 32, DOMSEP_PKHASH)
+
+  return (vec_s, z, pk, pkh)
+
+fn CompressToR10(v: VecR13) -> VecR10:
+  let h1 = make_r13([4u13; 256])
+  let h = make_vec13([h1; ℓ])
+  let s = (v + h) >> 3
+  return (s as VecR10)
+
+fn CompressToRt(r: R10) -> Rt:
+  let h1 = make_r10([4u10; 256])
+  let s = (r + h1) >> (10 - t)
+  return (s as Rt)
+
+fn DecodeMsg(r: R10) -> R1:
+  let h2 = make_r10([2^8 - 2^(10-t-1) + 4; 256])
+  let s = (r + h2) >> 9
+  return (s as R1)
+
+fn GenMat(seed: [u8; 32]) -> MatR13:
+  let A: [[R13; ℓ]; ℓ]
+  for i in 0u8..ℓ:
+    for j in 0u8..ℓ:
+      let buf = TurboSHAKE128(seed || i || j, 256*13/8, DOMSEP_GENMAT)
+      A[i][j] = deserialize_elem(13, buf)
+  return make_mat13(A)
+
+fn GenSecret(seed: [u8; 32]) -> VecR13:
+  let s: [R13; ℓ]
+  for i in 0u8..ℓ:
+    let buf = TurboSHAKE256(seed || i, μ*256/8, DOMSEP_GENSEC)
+    let vals = bit_slices(buf)
+    let r: [u13; 256]
+    for k in 0..256:
+      # Recall subtraction is wrapping
+      r[k] = hamming(vals[2*k]) - hamming(vals[2*k+1])
+    s[i] = make_r13(r)
+  return make_vec13(s)
+
+# Serializes an element of Rn (for any choice n=13,10,1,t)
+fn serialize_elem(n: ℤ, r: Rn) -> [u8; n*256/8]:
+  let a = canonical_coeffs(r)
+
+  let all_bits: [bool; n*256]
+  for i in 0..256:
+    all_bits[n*i..n*(i+1)] = to_bits_le(n, a[i])
+
+  let out: [u8; 32*n]
+  for i in 0..32*n:
+    out[i] = from_bits_le(8, all_bits[8*i..8*(i+1)])
+  return out
+
+# Serializes an element of VecRn (for any choice n=13,10,1,t)
+fn serialize_vec(n: ℤ, v: VecRn) -> [u8; ℓ*n*256/8]:
+  let out: [u8; ℓ*n*32]
+  for i in 0..ℓ:
+    out[n*32*i..n*32*(i+1)] = serialize_elem(n, v[i])
+  return out
+
+# Deserializes an element of Rn (for any choice n=13,10,1,t)
+fn deserialize_elem(n: ℤ, bytes: [u8; n*256/8]) -> Rn:
+  let all_bits: [bool; n*256]
+  for i in 0..n*32:
+    all_bits[8*i..8*(i+1)] = to_bits_le(8, bytes[i])
+
+  let coeffs: [un; 256]
+  for i in 0..256:
+    coeffs[i] = from_bits_le(n, all_bits[n*i..n*(i+1)])
+  return make_rn(coeffs)
+
+# Deserializes an element of VecRn (for any choice n=13,10,1,t)
+fn deserialize_vec(n: ℤ, bytes: [u8; ℓ*n*256/8]) -> VecRn:
+  let elems: [Rn; ℓ]
+  for i in 0..ℓ:
+    elems[i] = deserialize_elem(n, bytes[n*32*i..n*32*(i+1)])
+  return make_vecn(elems)
+
+# Reinterprets a bytestring as a sequence of bitstrings of length μ/2
+fn bit_slices(bytes: [u8; μ*256/8]) -> [[bool; μ/2]; 512]:
+  let all_bits: [bool; μ*256]
+  for i in 0..μ*32:
+    all_bits[8*i..8*(i+1)] = to_bits_le(8, bytes[i])
+
+  let out: [[bool; μ/2]; 512]
+  for i in 0..512:
+    out[i] = all_bits[i*μ/2..(i+1)*μ/2]
+  return out
+
+# Returns the number of set bits in b
+fn hamming(b: [bool; μ/2]) -> u13:
+  let mut weight = 0u13
+  for i in 0..μ/2:
+    if b[i]:
+      weight += 1
+  return weight
+```
+
+# Parameter Sets
+
+We define three security levels for Kopis: Kopis-512, Kopis-768, and Kopis-1024, referring to dimension of the public key vector over `ℤ/2¹⁰ℤ`:
+
+|Name       | Parameters     | `PK_SIZE` | `CT_SIZE` | `SK_SIZE` |
+|---------- |----------------|-----------|-----------|-----------|
+|Kopis-512  | `ℓ=2 t=3 μ=10` | 672       | 736       | 32        |
+|Kopis-768  | `ℓ=3 t=4 μ=8`  | 992       | 1088      | 32        |
+|Kopis-1024 | `ℓ=4 t=6 μ=6`  | 1312      | 1472      | 32        |
